\documentclass[fleqn]{article}
\usepackage{amsmath}
\usepackage[margin = 1 in]{geometry}

\title{Shaum series - Complex Variable - Problem 1.130}
\author{Md. Mesbahose Salekeen}

\begin{document}
\maketitle

prove that 

$$\cos^{n}(\phi)= \frac{1}{2^{n-1}}\{\cos n\phi+\cos(n-2)\phi+\frac{n(n-1)}{2!}\cos(n-4)\phi+..........+R_{n}\}$$

where \[ \hspace{48pt} R_{n} = \begin{cases} 
      \frac{n!}{[\frac{(n-1)}{2}]![\frac{(n+1)}{2}]!}\cos(\phi) & \text{if n is odd} \\
      \frac{n!}{2[(\frac{n}{2})!]^{2}} & \text{if n is even} 
   \end{cases}
\]

\textbf{Proof}

We know,
$$\cos(\phi) = \frac{1}{2}\bigg(e^{i\phi}+e^{-i\phi}\bigg)$$

so 
$$\hspace{10pt}\cos^{n}(\phi) = \frac{1}{2^{n}}\bigg(e^{i\phi}+e^{-i\phi}\bigg)^{n}$$


\begin{align*}
\cos^{n}(\phi) &= \frac{1}{2^{n}}\bigg(e^{i\phi}+e^{-i\phi}\bigg)^{n}\\
            &= \frac {1}{2^{n}}\{^{n}C_{0}e^{ni\phi}+^{n}C_{1}e^{(n-1)i\phi}e^{-i\phi}+^{n}C_{2}e^{(n-2)i\phi}e^{-2i\phi}+...........\\
            &+^{n}C_{n-1}e^{\{n-(n-1)\}i\phi}e^{-(n-1)i\phi}+^{n}C_{n}e^{i\phi}e^{-ni\phi}\}\\
            &= \frac{1}{2^{n}}\{e^{ni\phi}+ne^{(n-2)i\phi}+\frac{n(n-1)}{2!}e^{(n-4)i\phi}+.............+ne^{-(n-2)i\phi}+e^{-in\phi}\}\\
            &=\frac{1}{2^{n}}\sum_{k=0}^{n}\binom{n}{k}e^{(n-2k)i\phi}
\end{align*}

so 

$$\cos^{n}(\phi)=\frac{1}{2^{n}}\sum_{k=0}^{n}\binom{n}{k}e^{(n-2k)i\phi}....................(1)$$

from law of combination we know,

$$^{n}C_{r} = ^{n}C_{n-r}$$

so 

$$\frac{1}{2^{n}}\sum_{k=0}^{n}\binom{n}{k}e^{(n-2k)i\phi} = \frac{1}{2^{n}}\sum_{k=0}^{n}\binom{n}{n-k}e^{(2k-n)i\phi}$$

which gives

\begin{align*}
\cos^{n}(\phi) &=\frac{1}{2^{n}}\sum_{k=0}^{n}\binom{n}{n-k}e^{(2k-n)i\phi}\\
			   &= \frac{1}{2^{n}}\sum_{k=0}^{n}\binom{n}{n-k}e^{-(n-2k)i\phi}\\
			   &= \frac{1}{2^{n}}\sum_{k=0}^{n}\binom{n}{k}e^{-(n-2k)i\phi}
\end{align*}

\vspace{1 cm}

$\frac{(1)+(2)}{2}$ gives

\begin{align*}
\cos^{n}(\phi) &= \frac{1}{2^{n}}\{\sum_{k=0}^{n}\frac{1}{2}\bigg(\binom{n}{k}e^{(n-2k)i\phi}+\sum_{k=0}^{n}\binom{n}{k}e^{-(n-2k)i\phi}\}\bigg)\\
			   &=\frac{1}{2^{n}}\{\sum_{k=0}^{n}\binom{n}{k}\cos(n-2k)\phi\}\\
			   &=\frac{1}{2^{n}}\{\cos(n\phi)+n\cos(n-2)\phi+ \frac{n(n-1)}{2!}\cos(n-4)\phi+........+n\cos(n-2)\phi+\cos(n\phi)\}\\
			   & \hspace{340pt}..............(3)
\end{align*}

$\text{if n is odd there will be n+1 even terms}$

\begin{table}[hbtp]
\caption{odd relationship}
\begin{center}
\begin{tabular}{|l|l|l|l|l|}

\hline
0 & 1 & 2 &..... &$\frac{n-1}{2}$\\
\hline
n & n-1 & n-2 &...&$\frac{n+1}{2}$\\
\hline

\end{tabular}
\end{center}
\end{table}

$\text{from..(3) we get}$

\begin{align*}
\cos^{n}(\phi) &= \frac{1}{2^{n}}\{\cos(n\phi)+n\cos(n-2)\phi+\frac{n(n-1)}{2!}\cos(n-4)\phi+....+\\
			   & \binom{n}{\frac{n-1}{2}}\cos\{n-2\frac{(n-1)}{2}\}+ \binom{n}{\frac{n+1}{2}}\cos\{n-2\frac{(n+1)}{2}\}+\\
			   &.......+n\cos(n-2)\phi+\cos(n\phi)\}.........................(4)\\	   
\end{align*}

Now $$\binom{n}{(\frac{n-1}{2})} = \binom{n}{(\frac{n+1}{2})}=\frac{n!}{(\frac{n-1}{2})!(\frac{n+1}{2})!}$$

$\text{from ...(4) we get}$

\begin{align*}
\cos^{n}(\phi) &= \frac{1}{2^{n-1}} \{\cos(n\phi)+n\cos(n-2)\phi+\frac{n(n-1)}{2}\cos(n-4)\phi+...............+\frac{n!}{(\frac{n-1}{2})!(\frac{n+1}{2})!}\cos(\phi)\}\\
\end{align*}

$\text{if n is even there will be n+1 odd terms}$

\begin{table}[hbtp]
\caption{even relationship}
\begin{center}
\begin{tabular}{|l|l|l|l|l|l|}

\hline
0 & 1 & 2 &..... &$\frac{n}{2}-1$ & $\frac{n}{2}$\\
\hline
n & n-1 & n-2 &...&$\frac{n}{2}+1$ & \\
\hline

\end{tabular}
\end{center}
\end{table}

\vspace{1.5 in}

$\text{from ....(3) we get}$

\begin{align*}
\cos^{n}(\phi) &= \frac{1}{2^{n}}\{\cos(n\phi)+n\cos(n-2)\phi+\frac{n(n-1)}{2!}\cos(n-4)\phi+....+\\
			   & \frac{n!}{[(\frac{n}{2})!]^{2}}+.......+n\cos(n-2)\phi+\cos(n\phi)\}\\	
			   &= \frac{1}{2^{n-1}}\{\cos(n\phi)+n\cos(n-2)\phi+\frac{n(n-1)}{2!}\cos(n-4)\phi+......\\
			   &..+\frac{n!}{[(\frac{n}{2})!]^{2}} \}   
\end{align*}

$$\text{\textbf{[Proved]}}$$

\end{document}