\documentclass[fleqn]{article}
\usepackage{amsmath}
\usepackage[margin = 1 in]{geometry}

\begin{document}

$\text{Prove that for any integer }m \leq 1$

\begin{align*}
(z+a)^{2m}-(z-a)^{2m} &= 4maz\prod_{k=1}^{m-1}\{z^{2}+a^{2}cot{(\frac{k\pi}{2m})}\}
\end{align*}

\textbf{Solution}

\vspace{12pt}
$\text{From roots of }(z+a)^{2m} = (z-a)^{2m}$

\begin{align*}
\bigg(\frac{z+a}{z-a}\bigg)^{2m} &= 1
\end{align*}

Next

$$(\frac{z+a}{z-a}) = e^{(\frac{2\pi k}{2m})i}$$
$$\Rightarrow(\frac{z}{a})=\frac{e^{\frac{\pi k}{m}}+1}{e^{\frac{\pi k}{m}}-1}$$
$$\Rightarrow z = a\frac{e^{\frac{\pi k}{m}}+1}{e^{\frac{\pi k}{m}}-1}$$

Here

\begin{align*}
z &= a\cdot \frac{(e^{\frac{\pi k}{m}}+1)(e^{-\frac{\pi k}{m}}-1)}{(e^{\frac{\pi k}{m}}-1)(e^{-\frac{\pi k}{m}}-1)}\\
&=a \cdot \frac{-2i\sin(\frac{\pi k}{m})}{2-2\cos(\frac{\pi k}{m})}\\
&=ia\cot(\frac{\pi k}{2m})......k=\pm1,\pm2,\pm3,.....,\pm(m-1)
\end{align*}

So

\begin{align*}
(z+a)^{2m}-(z-a)^{2m} &= Cz\prod_{k=1}^{m-1}\{z-ia\cot(\frac{\pi k}{2m})\}\{z+ia\cot(\frac{\pi k}{m})\}\\
				&=Cz\prod_{k=1}^{m-1}\{z^{2}+a^{2}\cot^{2}(\frac{\pi k}{2m})\}..................(1)\\				
\end{align*}

From binomial expansion

\begin{align*}
(z+a)^{2m}-(z-a)^{2m} &= (^{2m}C_{0}z^{2m}+^{2m}C_{1}z^{2m-1}a+^{2m}C_{2}z^{2m-2}a^{2}+.....+^{2m}C_{2m-1}za^{2m-1}\\
&+^{2m}C_{2m}a^{2m}) - (^{2m}C_{0}z^{2m}-^{2m}C_{1}z^{2m-1}a+^{2m}C_{2}z^{2m-2}a^{2}\\
&.....-^{2m}C_{2m-1}za^{2m-1}+^{2m}C_{2m}a^{2m})\\
&=2\bigg(^{2m}C_{1}z^{2m-1}a+^{2m}C_{3}z^{2m-3}a^{3}+........+^{2m}C_{2m-1}za^{2m-1}\bigg)\\
&=2\cdot 2m\cdot a\cdot z\bigg(z^{2m-2}+\frac{(2m-1)(2m-2)}{3!}z^{2m-4}a^{2}+........+a^{2m-2}\bigg).........(2)\\
\end{align*}

From (1) and  (2) equating the right side, we get
$$C= 4ma$$

putting $C$ in (1) we get 

\begin{align*}
(z+a)^{2m}-(z-a)^{2m} &= 4maz\prod_{k=1}^{m-1}\{z^{2}+a^{2}cot{(\frac{k\pi}{2m})}\}
\end{align*}

\begin{center}
[Proved]
\end{center}

\end{document}