\documentclass[fleqn]{article}
\usepackage{amsmath}
\usepackage[margin = 1 in]{geometry}

\begin{document}
\text{Prove that }
$$\prod_{k=1}^{n-1}\sin\bigg(\frac{k \pi}{n}\bigg) = \frac{n}{2^{n-1}}$$

\begin{align*}
L.H.S &= \prod_{k=1}^{n-1}\sin\bigg(\frac{k \pi}{n}\bigg)\\
	  &=\prod_{k=1}^{n-1}\bigg(\frac{e^{\frac{k \pi}{n}i}-e^{-\frac{k \pi}{n}i}}{2i}\bigg)\\
	  &=\frac{1}{(2i)^{n-1}}\prod_{k=1}^{n-1}e^{-\frac{k \pi}{n}i}\bigg(e^{\frac{2k\pi}{n}i}-1\bigg)\\
	  &=\frac{1}{(2i)^{n-1}}\prod_{k=1}^{n-1}e^{-\frac{k \pi}{n}i}\prod_{k=1}^{n-1}\bigg(e^{\frac{2k\pi}{n}i}-1\bigg)...................(1)
	  \label{eq:1}
\end{align*}
Now 

\begin{align*}
\prod_{k=1}^{n-1}e^{-\frac{k \pi}{n}i} &= e^{-\frac{\pi i}{n}(1+2+3+.............+n-1)}\\
									   &= e^{-\frac{\pi}{n}\frac{n(n-1)i}{2}}\\
									   &= e^{-\frac{\pi (n-1)i}{2}}\\
									   &= e^{\frac{\pi}{2}i}\cdot e^{-\frac{\pi n}{2}i}\\
									   &= ie^{-\frac{\pi n}{2}i}\\
\end{align*}

$$\text{if n = 1..........................................} e^{-\frac{\pi}{2}i} = -i = (-1)^{1}(i)^{1}$$
$$\text{if n = 2..........................................} e^{-\frac{2\pi}{2}i} = -1 = (-1)^{2}(i)^{2}$$
$$\text{if n = 3..........................................} e^{-\frac{3\pi}{2}i} = i = (-1)^{3}(i)^{3}$$
$$\text{if n = 4..........................................} e^{-\frac{4\pi}{2}i} = 1 = (-1)^{4}(i)^{4}$$
$$...................................................................$$
$$\text{if n = n..........................................} e^{-\frac{n\pi}{2}i} = .. = (-1)^{n}(i)^{n}$$

So

$$\prod_{k=1}^{n-1}\sin\bigg(\frac{k \pi}{n}\bigg) = (-1)^{n}i^{n+1}$$

\vspace{155pt}

from ....(1) we get

\begin{align*}
\prod_{k=1}^{n-1}\sin\bigg(\frac{k \pi}{n}\bigg) &= \frac{1}{(2i)^{n-1}}(-1)^{n}i^{n+1}\prod_{k=1}^{n-1}\bigg(e^{\frac{2k\pi}{n}i}-1\bigg)\\
												 &=2^{1-n}(-1)^{n+1}\prod_{k=1}^{n-1}\bigg(e^{\frac{2k\pi}{n}i}-1\bigg)\\
												 &=(-2)^{1-n}(-1)^{n-1}\prod_{k=1}^{n-1}\bigg(1-e^{\frac{2k\pi}{n}i}\bigg)\\
												 &=2^{1-n}\prod_{k=1}^{n-1}\bigg(1-e^{\frac{2k\pi}{n}i}\bigg).....................(2)\\
\end{align*}

considering roots of $z^{n} = 1$

$$z^{n} = e^{2k\pi i}......\text{k = 0,1,2,3.....n-1 (a total of n roots)}$$

So, the roots are

$$z = e^{\frac{2k\pi i}{n}}.........\text{k = 0,1,2,......,(n-1)}$$

$$z^{n} - 1 = \prod_{k = 0}^{n-1}(z - e^{\frac{2k\pi i}{n}})$$

Using binomial theorem, we get

$$(z-1)(1+z+z^{2}+......+z^{n-1} = (z-1)\prod_{k = 1}^{n-1}(z - e^{\frac{2k\pi i}{n}})$$

$$1+z+z^{2}+.........+z^{n-1} = \prod_{k = 1}^{n-1}(z - e^{\frac{2k\pi i}{n}})$$

putting $z = 1$

$$n = \prod_{k = 1}^{n-1}(z - e^{\frac{2k\pi i}{n}})$$

from...........(2) we get

$$\prod_{k=1}^{n-1}\sin\bigg(\frac{k \pi}{n}\bigg) = \frac{n}{2^{n-1}}$$

\end{document}